Code cleanup

kore/src/Syntax.v
@@ -10,6 +10,20 @@ Section Syntax.
 
   Context {Σ : Signature}.
 
+  (**
+    This definition is the abstract syntax of Kore, in the
+    dependently-typed setting. It also utilises a locally-
+    nameless variable presentation:
+
+    ```
+    Pattern [s₁, ..., sₙ] [S₁, ..., Sₘ] s
+    ```
+
+    Should be understood as a pattern of sort `s`, which has
+    `n` free (dangling) de Bruijn _element_ variables of sorts
+    s₁, ..., sₙ, and `m` free de Bruijn _set_ variables of 
+    sorts S₁, ..., Sₙ.
+  *)
   Inductive Pattern : list sort -> list sort -> sort -> Type :=
   | kore_bevar {ex mu : list sort} {s : sort}
                (idx : InTy s ex) : Pattern ex mu s
@@ -20,9 +34,10 @@ Section Syntax.
   | kore_fsvar {ex mu : list sort} {s : sort}
                (X : svar s) : Pattern ex mu s
 
-  | kore_app   {ex mu : list sort} (* (ss : list sort) (explicit app arg sort)? *)
+  | kore_app   {ex mu : list sort}
                (σ : symbol)
-               (args : hlist (Pattern ex mu) (arg_sorts σ)) : Pattern ex mu (ret_sort σ)
+               (args : hlist (Pattern ex mu) (arg_sorts σ))
+               : Pattern ex mu (ret_sort σ)
 
   | kore_bot   {ex mu : list sort}
                (s : sort) : Pattern ex mu s
@@ -68,6 +83,7 @@ Section Syntax.
   | kore_rewrites (* (s : sort) ? *) (φ1 φ2 : Pattern)
   | kore_dv       (s : sort) (s : string) *).
 
+  (** Custom-made recursion and induction principles: *)
   Section pat_rect.
     Variables
       (P : forall {ex mu s}, Pattern ex mu s -> Type).
@@ -273,42 +289,6 @@ Module Notations.
   Notation "p1 '⊆k{' s2 '}' p2" := (kore_in s2 p1 p2) (at level 68, format "p1  '⊆k{' s2 '}'  p2", left associativity) : kore_scope.
   Check (⊥{_} ⊆k{_} Top{_})%kore.
 
-(*   Notation "''" := (kore_is_sort s).
-  Notation := (kore_is_predicate s p).
-  Notation := (kore_is_nonempty_sort s). *)
-
-  (* Notation "'mu' s , p" := (kore_mu s p) (at level 80).
-  Check mu Nat, ⊥.
-  Notation "'nu' s , p" := (kore_nu s p) (at level 80).
-  Check nu Nat, ⊥. *)
-
-  (* Notation "'•(' s ')' p"    := (kore_next s p) (at level 30, format "'•(' s ')'  p") : kore_scope.
-  Check •(Nat) ⊥.
-  Notation "'○(' s ')' p"    := (kore_all_path_next s p) (at level 71, format "'○(' s ')'  p") : kore_scope.
-  Check ○(Nat) ⊥.
-  Notation "'⋄(' s ')' p"    := (kore_eventually s p) (at level 71, format "'⋄(' s ')'  p") : kore_scope.
-  Check ⋄(Nat) ⊥.
-  Notation "'⋄ʷ(' s ')' p"   := (kore_weak_eventually s p) (at level 71, format "'⋄ʷ(' s ')'  p") : kore_scope.
-  Check ⋄ʷ(Nat) ⊥.
-(*   Notation "s"       := (kore_well_founded s) (at level 71) : kore_scope. *)
-(*   Notation ""       := (kore_well_founded_alt s) (at level 71) : kore_scope. *)
-  Notation "'⊞(' s ')' p"    := (kore_always s p) (at level 71, format "'⊞(' s ')'  p") : kore_scope. (* □ is taken by application contexts *)
-  Check ⊞(Nat) ⊥.
-  Notation "p '=(' s ')=>' q"  := (kore_rewrites s p q) (at level 81, format "p  '=(' s ')=>'  q") : kore_scope.
-  Check ⊥ =(Nat)=> Top.
-  Notation "p '=(' s ')=>*' q" := (kore_rewrites_star s p q) (at level 81, format "p  '=(' s ')=>*'  q") : kore_scope.
-  Check ⊥ =(Nat)=>* Top.
-  Notation "p '=(' s ')=>⁺' q" := (kore_rewrites_plus s p q) (at level 81, format "p  '=(' s ')=>⁺'  q") : kore_scope.
-  Check ⊥ =(Nat)=>⁺ Top.
-
-(* These probably don't need notations:
-  Notation "" := (kore_one_path_reaches_star s p1 p2).
-  Notation := (kore_one_path_reaches_plus s p1 p2). *)
-  Notation "'↺(' s ')' p" := (kore_circularity s p) (at level 71, format "'↺(' s ')'  p").
-  Check ↺(Nat) ⊥.
-  Notation "s ⇑" := (kore_non_terminating s) (at level 90).
-  Check ⊥ ⋅ ⊥ ⇑. *)
-
 End Notations.
 
 Section DerivedNotations.
@@ -331,198 +311,21 @@ Section DerivedNotations.
     ) (kore_bevar In_nil)).
 
 
+  (* Notation "'•(' s ')' p"    := (kore_next s p) (at level 30, format "'•(' s ')'  p") : kore_scope.
+  Check •(Nat) ⊥.
+  Notation "'○(' s ')' p"    := (kore_all_path_next s p) (at level 71, format "'○(' s ')'  p") : kore_scope.
+  Check ○(Nat) ⊥.
+  Notation "'⋄(' s ')' p"    := (kore_eventually s p) (at level 71, format "'⋄(' s ')'  p") : kore_scope.
+  Check ⋄(Nat) ⊥.
+  Notation "'⋄ʷ(' s ')' p"   := (kore_weak_eventually s p) (at level 71, format "'⋄ʷ(' s ')'  p") : kore_scope.
+  Check ⋄ʷ(Nat) ⊥.
+  Notation "p '=(' s ')=>' q"  := (kore_rewrites s p q) (at level 81, format "p  '=(' s ')=>'  q") : kore_scope.
+  Check ⊥ =(Nat)=> Top.
+  Notation "p '=(' s ')=>*' q" := (kore_rewrites_star s p q) (at level 81, format "p  '=(' s ')=>*'  q") : kore_scope.
+  Check ⊥ =(Nat)=>* Top.
+  Notation "p '=(' s ')=>⁺' q" := (kore_rewrites_plus s p q) (at level 81, format "p  '=(' s ')=>⁺'  q") : kore_scope.
+  Check ⊥ =(Nat)=>⁺ Top. *)
+
 End DerivedNotations.
 
-(*
-Section Sortedness.
-  Import Notations.
-  Context {Σ : Signature}.
-  Open Scope kore_scope.
-
-  Definition shift {T : Set} (f : nat -> T) (d : T)
-    : nat -> T :=
-    fun n => match n with
-              | O => d
-              | S n' => f n'
-             end.
-
-  Definition update {T : Set} (n : nat) (d : T) (f : nat -> T)
-    : nat -> T :=
-    fun m => if decide (n = m) then d else f m.
-
-  Fixpoint app_ws (well_sorted : sort -> Pattern -> bool)
-                  (φs : list Pattern)
-                  (ss : list sort) {struct φs} :=
-    match φs, ss with
-    | [], [] => true
-    | φ::φs, s::ss => well_sorted s φ &&
-                      app_ws well_sorted φs ss
-    | _, _ => false
-    end.
-
-  Fixpoint well_sorted
-    (esorts : nat -> option sort)
-    (ssorts : nat -> option sort)
-    (s : sort)
-    (p : Pattern) {struct p} : bool :=
-    match p with
-     | kore_bot s => true
-     | kore_top s => true
-     | kore_bevar dbi => decide (esorts dbi = Some s)
-     | kore_bsvar dbi => decide (ssorts dbi = Some s)
-     | kore_fevar x => decide (evar_sort x = s)
-     | kore_fsvar X => decide (svar_sort X = s)
-     | kore_imp φ1 φ2 | kore_iff φ1 φ2
-     | kore_and φ1 φ2 | kore_or φ1 φ2
-       => well_sorted esorts ssorts s φ1 &&
-          well_sorted esorts ssorts s φ2
-     | kore_not φ => well_sorted esorts ssorts s φ
-     | kore_app σ args =>
-        decide (s = ret_sort σ) &&
-        app_ws (well_sorted esorts ssorts) args (arg_sorts σ)
-     | kore_exists s0 φ | kore_forall s0 φ =>
-        well_sorted (shift esorts (Some s0)) ssorts s φ
-     | kore_mu s0 φ | kore_nu s0 φ =>
-        well_sorted esorts (shift ssorts (Some s0)) s φ
-     | kore_ceil s1 s2 φ | kore_floor s1 s2 φ
-        => well_sorted esorts ssorts s1 φ &&
-           decide (s2 = s)
-     | kore_equals s1 s2 φ1 φ2 | kore_in s1 s2 φ1 φ2
-        => well_sorted esorts ssorts s1 φ1 &&
-           well_sorted esorts ssorts s1 φ2 &&
-           decide (s2 = s)
-    end.
-
-  Definition default : nat -> option sort := fun _ : nat => None.
-
-  Definition is_weaker (f1 f2 : nat -> option sort) : Prop :=
-    forall n s, f2 n = Some s -> f1 n = Some s.
-
-  Notation "f '≤ₛ' g" := (is_weaker f g) (at level 50).
-
-  Lemma default_is_strongest :
-    forall f, f ≤ₛ default.
-  Proof.
-    intros f n σ H.
-    unfold default in H.
-    inversion H.
-  Defined.
-
-  Lemma is_weaker_refl :
-    forall f, f ≤ₛ f.
-  Proof.
-    intros. intro. intros.
-    assumption.
-  Defined.
-
-  Lemma is_weaker_shift :
-    forall f1 f2,
-      f1 ≤ₛ f2 ->
-      forall d,
-        (shift f1 d) ≤ₛ (shift f2 d).
-  Proof.
-    intros.
-    unfold is_weaker.
-    intros.
-    destruct n; simpl in *. assumption.
-    by apply H.
-  Defined.
-
-
-  Lemma shift_update :
-    forall {T: Set} (f : nat -> T) n d1 d2,
-      shift (update n d1 f) d2 =
-      update (S n) d1 (shift f d2).
-  Proof.
-    intros. unfold shift, update.
-    extensionality x.
-    destruct x; simpl. reflexivity.
-    destruct decide; simpl;
-    destruct decide; simpl; try lia; reflexivity.
-  Defined.
-
-  Lemma well_sorted_weaken :
-    forall φ s fe fe' fs fs',
-      fe' ≤ₛ fe ->
-      fs' ≤ₛ fs ->
-      well_sorted fe fs s φ ->
-      well_sorted fe' fs' s φ.
-  Proof.
-    induction φ using Pat_rect; intros * Hw1 Hw2 Hwf; try by constructor.
-    * simpl in *. destruct decide. 2: simpl in Hwf; congruence.
-      clear Hwf. apply Hw1 in e.
-      cbn. rewrite e. destruct decide; auto.
-    * simpl in *. assumption.
-    * simpl in *. destruct decide. 2: simpl in Hwf; congruence.
-      clear Hwf. apply Hw2 in e.
-      cbn. rewrite e. destruct decide; auto.
-    * simpl in *. assumption.
-    * simpl in *.
-      apply andb_split_1 in Hwf as H1. rewrite H1. simpl.
-      apply andb_split_2 in Hwf.
-      {
-        clear - H Hwf Hw1 Hw2.
-        remember (arg_sorts σ) as sorts.
-        clear Heqsorts. revert sorts Hwf.
-        induction args; simpl in *; intros.
-        + case_match; by auto.
-        + case_match. by auto.
-          subst.
-          inversion H. subst. erewrite H2. 2-3: eassumption.
-          2: by apply andb_split_1 in Hwf.
-          eapply IHargs. assumption.
-          by apply andb_split_2 in Hwf.
-      }
-    * simpl in *. eapply IHφ in Hwf; eassumption.
-    * simpl in *. apply andb_true_iff in Hwf as [Hwf1 Hwf2].
-      erewrite IHφ1; try eassumption.
-      erewrite IHφ2; try eassumption.
-      reflexivity.
-    * simpl in *. apply andb_true_iff in Hwf as [Hwf1 Hwf2].
-      erewrite IHφ1; try eassumption.
-      erewrite IHφ2; try eassumption.
-      reflexivity.
-    * simpl in *. apply andb_true_iff in Hwf as [Hwf1 Hwf2].
-      erewrite IHφ1; try eassumption.
-      erewrite IHφ2; try eassumption.
-      reflexivity.
-    * simpl in *. apply andb_true_iff in Hwf as [Hwf1 Hwf2].
-      erewrite IHφ1; try eassumption.
-      erewrite IHφ2; try eassumption.
-      reflexivity.
-    * simpl in *. eapply IHφ in Hwf. exact Hwf.
-      by apply is_weaker_shift.
-      assumption.
-    * simpl in *. eapply IHφ in Hwf. exact Hwf.
-      by apply is_weaker_shift.
-      assumption.
-    * simpl in *. eapply IHφ in Hwf. exact Hwf.
-      2: by apply is_weaker_shift.
-      assumption.
-    * simpl in *. eapply IHφ in Hwf. exact Hwf.
-      2: by apply is_weaker_shift.
-      assumption.
-    * simpl in *.
-      erewrite IHφ; try eassumption.
-      simpl. apply andb_split_2 in Hwf. assumption.
-      simpl. apply andb_split_1 in Hwf. assumption.
-    * simpl in *.
-      erewrite IHφ; try eassumption.
-      simpl. apply andb_split_2 in Hwf. assumption.
-      simpl. apply andb_split_1 in Hwf. assumption.
-    * simpl in *.
-      erewrite IHφ1; try eassumption.
-      erewrite IHφ2; try eassumption.
-      simpl. apply andb_split_2 in Hwf. assumption.
-      simpl. apply andb_split_1, andb_split_2 in Hwf. assumption.
-      simpl. apply andb_split_1, andb_split_1 in Hwf. assumption.
-    * simpl in *.
-      erewrite IHφ1; try eassumption.
-      erewrite IHφ2; try eassumption.
-      simpl. apply andb_split_2 in Hwf. assumption.
-      simpl. apply andb_split_1, andb_split_2 in Hwf. assumption.
-      simpl. apply andb_split_1, andb_split_1 in Hwf. assumption.
-  Defined.
-
-End Sortedness. *)
 
