kore/src/Semantics.v
@@ -18,218 +18,189 @@ Section Semantics.
 
   Section with_model.
 
-  Context {M : Model}.
-  Record Valuation : Type := {
-    evar_valuation {s : sort} (x : evar s) : carrier M s;
-    svar_valuation {s : sort} (X : svar s) : propset (carrier M s) ;
-  }.
+    Context {M : Model}.
+    Record Valuation : Type := {
+      evar_valuation {s : sort} (x : evar s) : carrier M s;
+      svar_valuation {s : sort} (X : svar s) : propset (carrier M s) ;
+    }.
 
-  Definition app_ext
-    (σ : symbol)
-    (args : @hlist _ (fun s => propset (carrier M s)) (arg_sorts σ))
-    : propset (carrier M (ret_sort σ)) :=
-  PropSet (
-    fun e => exists (l : @hlist _ (carrier M) (arg_sorts σ)),
-      pointwise_elem_of _ l args /\ e ∈ app M σ l
-  ).
+    Definition app_ext
+      (σ : symbol)
+      (args : @hlist _ (fun s => propset (carrier M s)) (arg_sorts σ))
+      : propset (carrier M (ret_sort σ)) :=
+    PropSet (
+      fun e => exists (l : @hlist _ (carrier M) (arg_sorts σ)),
+        pointwise_elem_of _ l args /\ e ∈ app M σ l
+    ).
 
 
-  Definition update_evar_val {s} (ev : evar s) (x : carrier M s) (val : Valuation) : Valuation.
-  Proof.
-    unshelve esplit.
-    intros s' ev'.
-    destruct (decide (s = s')).
-    destruct (decide (eq_rect s evar ev _ e = ev')).
-    exact (eq_rect s M x _ e).
-    1,2:exact (evar_valuation val ev').
-    exact (@svar_valuation val).
-  Defined.
+    Definition update_evar_val {s} (ev : evar s) (x : carrier M s) (val : Valuation) : Valuation.
+    Proof.
+      unshelve esplit.
+      intros s' ev'.
+      destruct (decide (s = s')).
+      destruct (decide (eq_rect s evar ev _ e = ev')).
+      exact (eq_rect s M x _ e).
+      1,2:exact (evar_valuation val ev').
+      exact (@svar_valuation val).
+    Defined.
 
-  Definition update_svar_val {s} (sv : svar s) (X : propset (carrier M s)) (val : Valuation) : Valuation.
-  Proof.
-    unshelve esplit.
-    exact (@evar_valuation val).
-    intros s' sv'.
-    destruct (decide (s = s')).
-    * destruct (decide (eq_rect s svar sv _ e = sv')).
-      - rewrite e in X. exact X.
-      - exact (svar_valuation val sv').
-    * exact (svar_valuation val sv').
-  Defined.
+    Definition update_svar_val {s} (sv : svar s) (X : propset (carrier M s)) (val : Valuation) : Valuation.
+    Proof.
+      unshelve esplit.
+      exact (@evar_valuation val).
+      intros s' sv'.
+      destruct (decide (s = s')).
+      * destruct (decide (eq_rect s svar sv _ e = sv')).
+        - rewrite e in X. exact X.
+        - exact (svar_valuation val sv').
+      * exact (svar_valuation val sv').
+    Defined.
 
-  Let OS s := PropsetOrderedSet (carrier M s).
-  Let  L s := PowersetLattice (carrier M s).
+    Let OS s := PropsetOrderedSet (carrier M s).
+    Let  L s := PowersetLattice (carrier M s).
 
-  Equations? eval {ex mu} {s} (ρ : Valuation) (φ : Pattern ex mu s) : propset (carrier M s) by wf (pat_size φ) :=
-    eval ρ (kore_bevar _) := empty ;
-    eval ρ (kore_fevar x) := {[evar_valuation ρ x]} ;
-    eval ρ (kore_bsvar _) := empty ;
-    eval ρ (kore_fsvar X) := svar_valuation ρ X ;
+    Equations? eval {ex mu} {s} (ρ : Valuation)
+                    (φ : Pattern ex mu s)
+                    : propset (carrier M s)
+                      by wf (pat_size φ) :=
+      eval ρ (kore_bevar _) := empty ;
+      eval ρ (kore_fevar x) := {[evar_valuation ρ x]} ;
+      eval ρ (kore_bsvar _) := empty ;
+      eval ρ (kore_fsvar X) := svar_valuation ρ X ;
 
-    eval ρ (kore_app σ l) := app_ext σ _ (*@hlist_rect _ _ (λ l _, hlist (propset ∘ M) l) hnil (λ _ _ a _ b, hcons (eval ρ a) b) _ l*)
+      eval ρ (kore_app σ l) := app_ext σ _ 
+      (* Map alternative, if wf ∘ pat_size would not be a requirement in the def.: *)
       (* (hmap (fun j (p : Pattern ex mu j) => eval ρ p) l) *) ;
 
-    eval ρ kore_bot         := empty ;
-    eval ρ kore_top         := ⊤ ;
-    eval ρ (kore_not φ)     := ⊤ ∖ (eval ρ φ) ;
-    eval ρ (kore_and φ1 φ2) := (eval ρ φ1) ∩ (eval ρ φ2) ;
-    eval ρ (kore_or φ1 φ2)  := (eval ρ φ1) ∪ (eval ρ φ2) ;
-    eval ρ (kore_imp φ1 φ2) := (⊤ ∖ (eval ρ φ1)) ∪ (eval ρ φ2) ;
-    eval ρ (kore_iff φ1 φ2) := (⊤ ∖ eval ρ φ1 ∪ eval ρ φ2) ∩
-                               (⊤ ∖ eval ρ φ2 ∪ eval ρ φ1) ;
+      eval ρ kore_bot         := empty ;
+      eval ρ kore_top         := ⊤ ;
+      eval ρ (kore_not φ)     := ⊤ ∖ (eval ρ φ) ;
+      eval ρ (kore_and φ1 φ2) := (eval ρ φ1) ∩ (eval ρ φ2) ;
+      eval ρ (kore_or φ1 φ2)  := (eval ρ φ1) ∪ (eval ρ φ2) ;
+      eval ρ (kore_imp φ1 φ2) := (⊤ ∖ (eval ρ φ1)) ∪ (eval ρ φ2) ;
+      eval ρ (kore_iff φ1 φ2) := (⊤ ∖ eval ρ φ1 ∪ eval ρ φ2) ∩
+                                 (⊤ ∖ eval ρ φ2 ∪ eval ρ φ1) ;
 
-    eval ρ (kore_exists s' φ) := (* ⊤ ≫= λ X, let o := fresh_evar s' φ in eval (update_evar_val o X ρ) (bevar_subst [] φ (kore_fevar o)) *)
-      let x := fresh_evar s' φ in
-        propset_fa_union (λ c,
-           eval (update_evar_val x c ρ)
-                (bevar_subst [] (kore_fevar x) φ)) ;
-    eval ρ (kore_forall s' φ) :=
-      let x := fresh_evar s' φ in
-        propset_fa_intersection (λ c,
-           eval (update_evar_val x c ρ)
-                (bevar_subst [] (kore_fevar x) φ)) ;
+      eval ρ (kore_exists s' φ) :=
+      (* Monadic alternative: 
+         ⊤ ≫= λ X, let o := fresh_evar s' φ in
+            eval (update_evar_val o X ρ) (bevar_subst [] φ (kore_fevar o)) *)
+        let x := fresh_evar s' φ in
+          propset_fa_union (λ c,
+             eval (update_evar_val x c ρ)
+                  (bevar_subst [] (kore_fevar x) φ)) ;
+      eval ρ (kore_forall s' φ) :=
+        let x := fresh_evar s' φ in
+          propset_fa_intersection (λ c,
+             eval (update_evar_val x c ρ)
+                  (bevar_subst [] (kore_fevar x) φ)) ;
 
-(*@LeastFixpointOf _ OS L
-                                  (fun S =>
-                                    let ρ' := (update_svar_val X S ρ) in
-                                    eval ρ' (ϕ'^{svar: 0 ↦ X})
-                                  )*)
+      eval ρ (kore_mu φ)     :=
+        let X := fresh_svar s φ in
+          @LeastFixpointOf _ (OS s) (L s) (fun S =>
+            eval (update_svar_val X S ρ)
+                 (bsvar_subst [] (kore_fsvar X) φ)
+          )
+       ;
+      eval ρ (kore_nu φ)     :=
+        let X := fresh_svar s φ in
+          @GreatestFixpointOf _ (OS s) (L s) (fun S =>
+            eval (update_svar_val X S ρ)
+                 (bsvar_subst [] (kore_fsvar X) φ)
+          );
 
-    eval ρ (kore_mu φ)     :=
-      let X := fresh_svar s φ in
-        @LeastFixpointOf _ (OS s) (L s) (fun S =>
-          eval (update_svar_val X S ρ)
-               (bsvar_subst [] (kore_fsvar X) φ)
-        )
-     ;
-    eval ρ (kore_nu φ)     :=
-      let X := fresh_svar s φ in
-        @GreatestFixpointOf _ (OS s) (L s) (fun S =>
-          eval (update_svar_val X S ρ)
-               (bsvar_subst [] (kore_fsvar X) φ)
-        );
+      eval ρ (kore_ceil φ)       := PropSet (λ _, ∃ c, c ∈ eval ρ φ) ;
+      eval ρ (kore_floor φ)      := PropSet (λ _, ∀ c, c ∈ eval ρ φ) ;
+      eval ρ (kore_equals φ1 φ2) := PropSet (λ _, (eval ρ φ1) = (eval ρ φ2)) ;
+      eval ρ (kore_in φ1 φ2)     := PropSet (λ _, (eval ρ φ1) ⊆ (eval ρ φ2)) ;
+    .
+    Proof.
+      1: { (* def. of eval ρ (σ ⋅ l) *)
+        simpl in *.
+        induction l.
+        * exact hnil.
+        * apply hcons.
+          - apply (eval _ _ _ ρ f). lia.
+          - apply IHl. intros.
+            apply (eval x0 x1 x2 x3 x4). lia.
+      }
+      (* wf ∘ pat_size constraints *)
+      all: try by simpl; lia.
+      1-2: rewrite (bevar_subst_size [] ex mu s s' φ x); constructor.
+      1-2: rewrite (bsvar_subst_size ex [] mu s s φ X); constructor.
+    Defined.
 
-    eval ρ (kore_ceil φ)       := PropSet (λ _, ∃ c, c ∈ eval ρ φ) ;
-    eval ρ (kore_floor φ)      := PropSet (λ _, ∀ c, c ∈ eval ρ φ) ;
-    eval ρ (kore_equals φ1 φ2) := PropSet (λ _, (eval ρ φ1) = (eval ρ φ2)) ;
-    eval ρ (kore_in φ1 φ2)     := PropSet (λ _, (eval ρ φ1) ⊆ (eval ρ φ2)) ;
-  .
-  Proof.
-    1: {
-      simpl in *.
+    (* simpler evaluation rule for σ ⋅ l *)
+    Lemma eval_app_simpl :
+      forall {ex mu} (σ : symbol) (l : hlist (Pattern ex mu) (arg_sorts σ)) (ρ : Valuation),
+        eval ρ (kore_app σ l) = app_ext σ (hmap (fun _ => eval ρ) l).
+    Proof.
+      intros.
+      simp eval. f_equal.
+      simpl in *. unfold eval_obligation_1. simpl. cbn.
       induction l.
-      * exact hnil.
-      * apply hcons.
-        - apply (eval _ _ _ ρ f). lia.
-        - apply IHl. intros.
-          apply (eval x0 x1 x2 x3 x4). lia.
-    }
-    all: try by simpl; lia.
-    1-2: rewrite (bevar_subst_size [] ex mu s s' φ x); constructor.
-    1-2: rewrite (bsvar_subst_size ex [] mu s s φ X); constructor.
-  Defined.
+      * reflexivity.
+      * rewrite IHl. reflexivity.
+    Defined.
 
-  Lemma eval_app_simpl :
-    forall {ex mu} (σ : symbol) (l : hlist (Pattern ex mu) (arg_sorts σ)) (ρ : Valuation),
-      eval ρ (kore_app σ l) = app_ext σ (hmap (fun _ => eval ρ) l).
-  Proof.
-    intros.
-    simp eval. f_equal.
-    simpl in *. unfold eval_obligation_1. simpl. cbn.
-    induction l.
-    * reflexivity.
-    * rewrite IHl. reflexivity.
-  Defined.
+    Lemma app_ext_singleton
+      {σ}
+      {args : hlist (propset ∘ M) (arg_sorts σ)}
+      (H : all_singleton args) :
+        app_ext σ args = app M σ (all_singleton_extract H).
+    Proof.
+      apply set_eq. split; intros.
+      unfold app_ext in H0.
+      destruct H0 as [? []].
+      replace (all_singleton_extract H) with x0. auto.
+      clear x H1. induction args.
+      simpl in *.
+      apply destruct_hnil.
+      simpl in H. destruct H. destruct s.
+      simpl in c. simpl.
+      epose proof destruct_hcons x0 as [[] ?]. rewrite y in H0.
+      simpl in H0. destruct H0. rewrite c in H. inversion H.
+      rewrite y. f_equal. apply IHargs. apply H0.
+      apply elem_of_PropSet. exists (all_singleton_extract H).
+      split. 2: auto. clear. induction args. simpl. split.
+      simpl in H. destruct H. destruct s. simpl in c. subst.
+      simpl. split. congruence.
+      apply IHargs.
+    Defined.
 
+    Lemma all_singleton_var_list {l} (vars : hlist evar l) ρ:
+      all_singleton (hmap (fun s (x : evar s) => {[evar_valuation ρ x]}) vars).
+    Proof.
+      induction vars; simpl.
+      * exact tt.
+      * apply pair. 2: exact IHvars.
+        eapply existT. reflexivity.
+    Defined.
 
-(*   Fixpoint HForall {J} {A : J -> Type}
-    (P : ∀ j, A j -> Prop)
-    {js : list J} (v : @hlist J A js) {struct v} : Prop :=
-    match v with
-    | hnil => True
-    | hcons x xs => P _ x ∧ HForall P xs
-    end.
-
-  Fixpoint HBiForall {J1 J2} {A1 : J1 -> Type} {A2 : J2 -> Type}
-    (P : ∀ j1 j2, A1 j1 -> A2 j2 -> Prop)
-    {js1 : list J1}
-    {js2 : list J2}
-    (v1 : @hlist J1 A1 js1) (v2 : @hlist J2 A2 js2)
-      {struct v1} : Prop :=
-    match v1, v2 with
-    | hnil, hnil => True
-    | hcons x xs, hcons y ys => P _ _ x y ∧ HBiForall P xs ys
-    | _, _ => False
-    end.*)
-
-  Lemma app_ext_singleton
-    {σ}
-    {args : hlist (propset ∘ M) (arg_sorts σ)}
-    (H : all_singleton args) :
-      app_ext σ args = app M σ (all_singleton_extract H).
-  Proof.
-    apply set_eq. split; intros.
-    unfold app_ext in H0.
-    destruct H0 as [? []].
-    replace (all_singleton_extract H) with x0. auto.
-    clear x H1. induction args.
-    simpl in *.
-    apply destruct_hnil.
-    simpl in H. destruct H. destruct s.
-    simpl in c. simpl.
-    epose proof destruct_hcons x0 as [[] ?]. rewrite y in H0.
-    simpl in H0. destruct H0. rewrite c in H. inversion H.
-    rewrite y. f_equal. apply IHargs. apply H0.
-    apply elem_of_PropSet. exists (all_singleton_extract H).
-    split. 2: auto. clear. induction args. simpl. split.
-    simpl in H. destruct H. destruct s. simpl in c. subst.
-    simpl. split. congruence.
-    apply IHargs.
-  Defined.
-
-  Lemma all_singleton_var_list {l} (vars : hlist evar l) ρ:
-    all_singleton (hmap (fun s (x : evar s) => {[evar_valuation ρ x]}) vars).
-  Proof.
-    induction vars; simpl.
-    * exact tt.
-    * apply pair. 2: exact IHvars.
-      eapply existT. reflexivity.
-  Defined.
-
-  Corollary eval_app_var_list :
-    forall ex mu (σ : symbol) (vars : hlist evar (arg_sorts σ)) (ρ : Valuation),
-      eval ρ (kore_app σ (var_list ex mu vars)) =
-        app M σ (all_singleton_extract (all_singleton_var_list vars ρ)).
-  Proof.
-    intros. rewrite eval_app_simpl.
-    rewrite <- app_ext_singleton.
-    (* there is a slight difference in the arguments *)
-    f_equal.
-    induction vars; simpl.
-    * reflexivity.
-    * rewrite IHvars. reflexivity.
-  Defined.
-
-(*   Lemma functional_symbol_eval :
-    forall (σ : symbol) (R : sort) (vars : hlist evar (arg_sorts σ)) (ρ : Valuation),
-      eval ρ (functional_symbol σ R vars) =
-        app M σ (all_singleton_extract (all_singleton_var_list vars ρ)).
-  Proof.
-    
-  Defined. *)
-
-(*   Lemma app_var_list_eval :
-    forall ex mu (σ : symbol) (vars : hlist evar (arg_sorts σ)) (M : Model) (ρ : Valuation),
-      eval ρ (kore_app σ (var_list ex mu vars)) =
-      app_ext σ (hmap (fun s (x : evar s) => {[evar_valuation ρ x]}) vars). *)
+    Corollary eval_app_var_list :
+      forall ex mu (σ : symbol) (vars : hlist evar (arg_sorts σ)) (ρ : Valuation),
+        eval ρ (kore_app σ (var_list ex mu vars)) =
+          app M σ (all_singleton_extract (all_singleton_var_list vars ρ)).
+    Proof.
+      intros. rewrite eval_app_simpl.
+      rewrite <- app_ext_singleton.
+      (* there is a slight difference in the arguments *)
+      f_equal.
+      induction vars; simpl.
+      * reflexivity.
+      * rewrite IHvars. reflexivity.
+    Defined.
 
 End with_model.
 
+  (** Satisfaction *)
   Definition satM {ex mu s} (φ : Pattern ex mu s) (M : Model) :=
     forall ρ, @eval M _ _ _ ρ φ = ⊤.
   Definition satT (Γ : Theory) (M : Model) :=
     forall p, p ∈ Γ -> @satM _ _ (projT1 p) (projT2 p) M.
 
+  (** Model construction based on curried application *)
   Program Definition mkModel
     (custom_carrier : sort → Set)
     (custom_app : forall (σ : symbol),
@@ -244,6 +215,8 @@ End with_model.
     app := fun σ => uncurry_n (custom_app σ)
   |}.
 
+  (** Model construction based on curried application of singleton-result
+      functions *)
   Definition mkModel_singleton
     (custom_carrier : sort → Set)
     (custom_app : forall (σ : symbol), foldr (λ c a, custom_carrier c -> a) (custom_carrier (ret_sort σ)) (arg_sorts σ))
@@ -255,6 +228,7 @@ End with_model.
     app := fun σ => singleton ∘ uncurry_n (custom_app σ)
   |}.
 
+  (** If a symbol is modeled by a function, it is consistent: *)
   Lemma functional_symbol_is_functional :
     forall (σ : symbol) (R : sort) (vars : hlist evar (arg_sorts σ)),
       forall (M : Model),
@@ -328,59 +302,65 @@ End with_model.
 
 End Semantics.
 
-  Ltac unfold_elem_of :=
+(** A tactic for deconstructing a concrete set. *)
+Ltac unfold_elem_of :=
+match goal with
+| [H : _ ∈ _ |- _]  => destruct H
+end.
+
+(** Case separation based on the value of variables. *)
+Ltac destruct_evar_val :=
+match goal with
+| [ |- context [evar_valuation ?ρ ?x] ] =>
+  let H := fresh "Val" in
+    destruct (evar_valuation ρ x) eqn:H
+end.
+
+(** This tactic is used to construct a proof for `all_singleton`. *)
+Ltac solve_dep_prods :=
   match goal with
-  | [H : _ ∈ _ |- _]  => destruct H
+  | [ |- ()] => exact tt
+  | [ |- prod (sigT _) _] =>
+    apply pair; [
+      eapply existT; reflexivity
+    |
+      solve_dep_prods
+    ]
   end.
 
-  Ltac destruct_evar_val :=
-  match goal with
-  | [ |- context [evar_valuation ?ρ ?x] ] =>
-    let H := fresh "Val" in
-      destruct (evar_valuation ρ x) eqn:H
-  end.
+Ltac solve_all_singleton :=
+match goal with
+| [ |- all_singleton _] => cbn; solve_dep_prods
+end.
 
-  Ltac solve_dep_prods :=
-    match goal with
-    | [ |- ()] => exact tt
-    | [ |- prod (sigT _) _] =>
-      apply pair; [
-        eapply existT; reflexivity
-      |
-        solve_dep_prods
-      ]
-    end.
+(* NOTE: This would be much more simple, if rewrite_stat innermost worked... *)
+(** This tactic rewrites `app_ext` (extension of application), if all
+    the arguments are singletons. The tactic rewrites the leftmost-innermost
+    occurrence of such `app_ext`. *)
+Ltac rewrite_app_ext_innnermost G :=
+match G with
+| context [@app_ext _ ?M ?σ ?args] =>
+  rewrite_app_ext_innnermost args (* This step is just to reach
+                                      the innermost app_ext *)
+  (* idtac "match" σ args *)
+| context [@app_ext _ ?M ?σ ?args] => (* This branch fails, if there is no
+                                   more app_exts, therefore
+                                   it succeeds for the last (innermost)
+                                   app_ext *)
+  (* idtac "last1" σ args; *)
+  (* let H := fresh "H" in
+  (* we explicitly rewrite: *)
+  unshelve (epose proof (@app_ext_singleton _ ImpModel σ args ltac:(solve_all_singleton)) as H);
+  (* idtac "last2" σ args; *)
+  rewrite H; (* erewrite does not work here, for some reason *)
+  clear H *)
+  rewrite (@app_ext_singleton _ M σ args ltac:(solve_all_singleton))
+end.
 
-  Ltac solve_all_singleton :=
-  match goal with
-  | [ |- all_singleton _] => cbn; solve_dep_prods
-  end.
-
-  (* This would be much more simple, if rewrite_stat innermost worked... *)
-  Ltac rewrite_app_ext_innnermost G :=
-  match G with
-  | context [@app_ext _ ?M ?σ ?args] =>
-    rewrite_app_ext_innnermost args (* This step is just to reach
-                                        the innermost app_ext *)
-    (* idtac "match" σ args *)
-  | context [@app_ext _ ?M ?σ ?args] => (* This branch fails, if there is no
-                                     more app_exts, therefore
-                                     it succeeds for the last (innermost)
-                                     app_ext *)
-    (* idtac "last1" σ args; *)
-    (* let H := fresh "H" in
-    (* we explicitly rewrite: *)
-    unshelve (epose proof (@app_ext_singleton _ ImpModel σ args ltac:(solve_all_singleton)) as H);
-    (* idtac "last2" σ args; *)
-    rewrite H; (* erewrite does not work here, for some reason *)
-    clear H *)
-    rewrite (@app_ext_singleton _ M σ args ltac:(solve_all_singleton))
-  end.
-
-  Ltac rewrite_app_ext :=
-  match goal with
-  | |- ?G => rewrite_app_ext_innnermost G; cbn
-  end.
+Ltac rewrite_app_ext :=
+match goal with
+| |- ?G => rewrite_app_ext_innnermost G; cbn
+end.
 
 
 Tactic Notation "deconstruct_elem_of_Theory" :=
@@ -388,6 +368,9 @@ Tactic Notation "deconstruct_elem_of_Theory" :=
   | [ H : _ ∈ _ |- _ ] => inversion H; subst; clear H
   end; clear; simpl.
 
+(** This tactic automatically simplifies the semantics of patterns with the
+    usual simplification tactic of `Equations`. However, in case of application
+    it uses a derived theorem. *)
 Tactic Notation "eval_helper" :=
   repeat
     match goal with
@@ -401,24 +384,27 @@ Tactic Notation "eval_helper" :=
     end.
 
 Tactic Notation "rewrite_singleton_all" :=
-    unshelve (rewrite_strat bottomup app_ext_singleton); [repeat esplit.. |].
+  unshelve (rewrite_strat bottomup app_ext_singleton); [repeat esplit.. |].
 
-  Ltac solve_functional_axiom :=
-  match goal with
-  | [ |- @eval _ ?M _ _ _ ?ρ (kore_exists _
-                  (kore_equals ?s (kore_app ?σ ?l)
-                               (kore_bevar In_nil))) = ⊤]
-                               (* ^- NOTE: this is a restriction on db index 0!!! This pattern checks whether the axiom is a functional axiom *) =>
-    let H := fresh "H" in
-    epose proof (functional_symbol_is_functional σ s (hmap (fun s p =>
-      match p with
-      | kore_fevar x => x
-      | _ => "_"%string
-      end) l) M);
-    apply H;
-    eexists;
-    reflexivity
-  end.
+(** This tactic proves the consistency of a functional axiom (based on the
+    `functional_symbol_is_functional` property). For this, it automatically
+    constructs a parameter list containing variables. *)
+Ltac solve_functional_axiom :=
+match goal with
+| [ |- @eval _ ?M _ _ _ ?ρ (kore_exists _
+                (kore_equals ?s (kore_app ?σ ?l)
+                             (kore_bevar In_nil))) = ⊤]
+                             (* ^- NOTE: this is a restriction on db index 0!!! This pattern checks whether the axiom is a functional axiom *) =>
+  let H := fresh "H" in
+  epose proof (functional_symbol_is_functional σ s (hmap (fun s p =>
+    match p with
+    | kore_fevar x => x
+    | _ => "_"%string
+    end) l) M);
+  apply H;
+  eexists;
+  reflexivity
+end.
 
 Add Search Blacklist "_elim".
 Add Search Blacklist "FunctionalElimination_".
